src/Env/Semantics.v
@@ -1,0 +1,113 @@
+From CoreErlang Require Export Env.Syntax.
+Import ListNotations.
+
+Inductive Frame : Set :=
+| FApp1 (l : list Exp) (* apply □(e₁, e₂, ..., eₙ) *)
+| FBIF1 (l : list Exp) (* call □(e₁, e₂, ..., eₙ) *)
+| FLet (e2 : Exp) (* let v = □ in e2 *)
+| FCase (p : Pat) (e2 e3 : Exp) (* if □ then e2 else e3 *)
+| FCons1 (e1 : Exp) (* [e1 | □] *)
+| FCons2 (v2 : Val) (* [□ | v2] *)
+
+| FApp2 (v : Val) (l : list Val) (el : list Exp)
+| FBIF2 (v : Val) (l : list Val) (el : list Exp).
+
+Definition FrameStack := list Frame.
+
+Definition Environment := list Val.
+
+Definition eval (f : Val) (l : list Val) : option Val :=
+match f with
+| VLit (Atom "+") =>
+  match l with
+  | [VLit (Int z1); VLit (Int z2)] => Some (VLit (Int (z1 + z2)))
+  | _ => None
+  end
+| _ => None
+end.
+
+Definition beta_reduce (f : Val) (params : list Val) : option (Environment * Exp) :=
+match f with
+| VClos Γ arity body =>
+    if Nat.eqb (length params) arity then
+      Some ((VClos Γ arity body) :: params ++ Γ, body)
+    else None
+| _ => None
+end.
+
+Reserved Notation "⟨ G , fs , e ⟩ --> ⟨ G' , fs' , e' ⟩" (at level 50).
+Inductive step : Environment -> FrameStack -> Exp -> Environment -> FrameStack -> Exp -> Prop :=
+(**  Reduction rules *)
+| red_bif0 Γ xs v res:
+  eval v [] = Some res ->
+  ⟨ Γ , (FBIF1 [])::xs, ˝v ⟩ --> ⟨ Γ, xs , res⟩
+
+| red_bif Γ xs e1 l v:
+  ⟨ Γ , (FBIF1 (e1::l))::xs, ˝v ⟩ --> ⟨ Γ, FBIF2 v [] l :: xs, e1 ⟩
+
+| step_bif_params Γ xs vl e1 el v v0:
+  ⟨ Γ , (FBIF2 v vl (e1::el))::xs, ˝v0 ⟩ --> ⟨ Γ, FBIF2 v (v0 :: vl) el :: xs, e1 ⟩
+
+| red_bif_params Γ xs vl v v0 res:
+  eval v (vl ++ [v0]) = Some res ->
+  ⟨ Γ , (FBIF2 v vl [])::xs, ˝v0 ⟩ --> ⟨ Γ, xs, res ⟩
+
+| red_app0 Γ xs v Γ' res:
+  beta_reduce v [] = Some (Γ', res) ->
+  ⟨ Γ , (FApp1 [])::xs, ˝v ⟩ --> ⟨ Γ', xs , res⟩
+
+| red_app Γ xs e1 l v:
+  ⟨ Γ , (FApp1 (e1::l))::xs, ˝v ⟩ --> ⟨ Γ, FApp2 v [] l :: xs, e1 ⟩
+
+| step_app_params Γ xs vl e1 el v v0:
+  ⟨ Γ , (FApp2 v vl (e1::el))::xs, ˝v0 ⟩ --> ⟨ Γ, FApp2 v (v0 :: vl) el :: xs, e1 ⟩
+
+| red_app_params Γ xs vl v v0 Γ' res:
+  beta_reduce v (vl ++ [v0]) = Some (Γ', res) ->
+  ⟨ Γ , (FApp2 v vl [])::xs, ˝v0 ⟩ --> ⟨ Γ', xs, res ⟩
+
+
+| red_let Γ val e2 xs :
+  ⟨ Γ , (FLet e2)::xs, ˝val ⟩ --> ⟨ val :: Γ, xs, e2 ⟩
+
+| red_case_true Γ e2 e3 v p xs l : 
+  match_pattern p v = Some l
+->
+  ⟨ Γ, (FCase p e2 e3)::xs, ˝v ⟩ --> ⟨ l ++ Γ, xs, e2 ⟩
+
+| red_case_false Γ e2 e3 p v xs :
+  match_pattern p v = None ->
+  ⟨ Γ, (FCase p e2 e3)::xs, ˝v ⟩ --> ⟨ Γ, xs, e3 ⟩
+
+| red_cons1 Γ xs v2 e1 :
+  ⟨ Γ, FCons1 e1::xs, ˝v2⟩ --> ⟨Γ,FCons2 v2::xs, e1 ⟩
+
+| red_cons2 Γ xs v2 v1 :
+  ⟨ Γ,FCons2 v2::xs, ˝v1⟩ --> ⟨Γ,xs, VCons v1 v2 ⟩
+
+(** Steps *)
+| step_let Γ xs e1 e2 : ⟨ Γ,xs, ELet e1 e2 ⟩ --> ⟨ Γ,(FLet e2)::xs, e1 ⟩
+| step_app Γ xs e el: ⟨ Γ,xs, EApp e el ⟩ --> ⟨ Γ,(FApp1 el)::xs, e ⟩
+| step_bif Γ fs name params:
+  ⟨Γ,fs, EBIF name params⟩ --> ⟨Γ,FBIF1 params :: fs, name⟩
+| step_case Γ xs e1 p e2 e3 : ⟨ Γ,xs, ECase e1 p e2 e3⟩ --> ⟨ Γ,(FCase p e2 e3)::xs, e1⟩
+| step_cons Γ xs e1 e2: ⟨ Γ,xs, ECons e1 e2 ⟩ --> ⟨ Γ,(FCons1 e1) :: xs, e2 ⟩
+
+(** Additional rules to handle environments *)
+| red_fun Γ xs vl e:
+  ⟨Γ, xs, EFun vl e⟩ --> ⟨Γ, xs, VClos Γ vl e⟩
+
+| red_var Γ xs x (val : Val) :
+  Γ !! x = Some val ->
+  ⟨Γ, xs, VVar x⟩ --> ⟨Γ, xs, ˝val⟩
+where "⟨ G , fs , e ⟩ --> ⟨ G' , fs' , e' ⟩" := (step G fs e G' fs' e').
+
+Reserved Notation "⟨ G , fs , e ⟩ -[ k ]-> ⟨ G' , fs' , e' ⟩" (at level 50).
+Inductive step_rt : Environment -> FrameStack -> Exp -> nat -> Environment -> FrameStack -> Exp -> Prop :=
+| step_refl Γ e Fs : ⟨ Γ, Fs, e ⟩ -[ 0 ]-> ⟨ Γ, Fs, e ⟩
+| step_trans Γ fs e Γ' fs' e' Γ'' fs'' e'' k:
+  ⟨ Γ, fs, e ⟩ --> ⟨ Γ', fs', e'⟩ -> ⟨Γ', fs', e'⟩ -[ k ]-> ⟨Γ'', fs'', e''⟩
+->
+  ⟨ Γ, fs, e ⟩ -[S k]-> ⟨Γ'', fs'', e''⟩
+where "⟨ G , fs , e ⟩ -[ k ]-> ⟨ G' , fs' , e' ⟩" := (step_rt G fs e k G' fs' e').
+
