src/Env/Syntax.v
@@ -1,0 +1,160 @@
+From CoreErlang Require Export SyntaxBasics.
+From stdpp Require Export base list.
+
+(** The syntax of expressions: *)
+Inductive Exp : Set :=
+| EExp (e : NonVal)
+| VVal (v : Val)
+
+with NonVal : Set :=
+(** Instead of multiple fun constructs (recursive and non-recursive), 
+    we use only recursive funs, which use the 0 DB-index as the recursive fun-exp *)
+| EFun    (vl : nat) (e : Exp)
+| EApp    (exp : Exp)     (l : list Exp)
+| ELet    (e1 e2 : Exp)
+(** Eliminator *)
+| ECase (e : Exp) (p : Pat) (e1 e2 : Exp)
+(** Lists *)
+| ECons (e1 e2 : Exp)
+(** Concurrency *)
+(* | EReceive (l : list (Pat * Exp)) *)
+| EBIF (e : Exp) (l : list Exp)
+
+with Val : Set :=
+| VLit    (l : Lit)
+| VPid    (p : PID)
+(** Variables and function identifiers are just indices.
+    TODO: In the future, function identifiers should include the arity too!
+*)
+| VVar    (n : nat)
+| VNil
+(** Recursive data structures which are values: *)
+| VCons (e1 e2 : Val)
+| VClos (Γ : list Val) (vl : nat) (e : Exp).
+
+Coercion EExp : NonVal >-> Exp.
+Coercion VVal : Val >-> Exp.
+Notation "˝ v" := (VVal v) (at level 11).
+Notation "° n" := (EExp n) (at level 11).
+
+
+Section correct_ind.
+
+Variables (P : Exp -> Prop) (PN : NonVal -> Prop) (PV : Val -> Prop)
+          (Q : list Exp -> Prop) (R : list Val -> Prop).
+
+Hypotheses
+  (HEExp : forall (nv : NonVal), PN nv -> P (EExp nv))
+  (HVVal : forall (v : Val), PV v -> P (VVal v))
+
+  (HNF_Fun : forall (vl : nat) (e : Exp), P e -> PN (EFun vl e))
+  (HNF_App : forall (e : Exp), P e -> forall (el : list Exp), Q el -> PN (EApp e el))
+  (HNF_Let : forall (e1 e2 : Exp), P e1 -> P e2 -> PN (ELet e1 e2))
+  (HNF_Case : forall (e : Exp) (p : Pat) (e1 e2 : Exp), P e -> P e1 -> P e2 -> PN (ECase e p e1 e2))
+  (HNF_Cons : forall (e1 e2 : Exp), P e1 -> P e2 -> PN (ECons e1 e2))
+  (HNF_EBIF : forall (e : Exp), P e -> forall (l : list Exp), Q l -> PN (EBIF e l))
+
+  (HV_Lit : forall (l : Lit), PV (VLit l))
+  (HV_Var : forall (n : nat), PV (VVar n))
+  (HV_Pid : forall (n : nat), PV (VPid n))
+  (HV_Nil : PV VNil)
+  (HV_Cons : forall (v1 v2 : Val), PV v1 -> PV v2 -> PV (VCons v1 v2))
+  (HV_Clos : forall (Gamma : list Val) (vl : nat) (e : Exp), R Gamma -> P e -> PV (VClos Gamma vl e))
+
+  (HQ_nil : Q [])
+  (HQ_cons : forall (e : Exp), P e -> forall (l : list Exp), Q l -> Q (e :: l))
+
+  (HR_nil : R [])
+  (HR_cons : forall (v : Val), PV v -> forall (l : list Val), R l -> R (v :: l)).
+
+Fixpoint Exp_ind2 (e : Exp) : P e :=
+  match e as x return P x with
+  | EExp nv => HEExp nv (NonVal_ind2 nv)
+  | VVal v => HVVal v (Val_ind2 v)
+  end
+
+with NonVal_ind2 (nv : NonVal) : PN nv :=
+  match nv as x return PN x with
+  | EFun vl e => HNF_Fun vl e (Exp_ind2 e)
+  | EApp e el => HNF_App e (Exp_ind2 e) el (
+      (fix l_ind (l' : list Exp) : Q l' :=
+         match l' as y return Q y with
+         | [] => HQ_nil
+         | v::xs => HQ_cons v (Exp_ind2 v) xs (l_ind xs)
+         end) el)
+  | ELet e1 e2 => HNF_Let e1 e2 (Exp_ind2 e1) (Exp_ind2 e2)
+  | ECase e p e1 e2 => HNF_Case e p e1 e2 (Exp_ind2 e) (Exp_ind2 e1) (Exp_ind2 e2)
+  | ECons e1 e2 => HNF_Cons e1 e2 (Exp_ind2 e1) (Exp_ind2 e2)
+  | EBIF e l => HNF_EBIF e (Exp_ind2 e) l (
+      (fix l_ind (l' : list Exp) : Q l' :=
+         match l' as y return Q y with
+         | [] => HQ_nil
+         | v::xs => HQ_cons v (Exp_ind2 v) xs (l_ind xs)
+         end) l)
+  end
+
+with Val_ind2 (v : Val) : PV v :=
+  match v as x return PV x with
+  | VLit l => HV_Lit l
+  | VVar n => HV_Var n
+  | VPid p => HV_Pid p
+  | VNil => HV_Nil
+  | VCons v1 v2 => HV_Cons v1 v2 (Val_ind2 v1) (Val_ind2 v2)
+  | VClos Gamma vl e => HV_Clos Gamma vl e (
+      (fix lV_ind (l' : list Val) : R l' :=
+         match l' as y return R y with
+         | [] => HR_nil
+         | v::xs => HR_cons v (Val_ind2 v) xs (lV_ind xs)
+         end) Gamma) (Exp_ind2 e)
+  end.
+
+End correct_ind.
+
+Fixpoint match_pattern (p : Pat) (e : Val) : option (list Val) :=
+match p with
+| PVar => Some [e]
+| PPid x => match e with
+            | VPid p => if Nat.eqb p x then Some [] else None
+            | _      => None
+            end
+| PNil => match e with
+          | VNil => Some []
+          | _    => None
+          end
+| PLit l0 => match e with
+             | VLit l => if lit_eqb l l0 then Some [] else None
+             | _      => None
+             end
+| PCons p1 p2 => 
+  match e with
+  | VCons v1 v2 =>
+    match match_pattern p1 v1, match_pattern p2 v2 with
+    | Some l1, Some l2 => Some (l1 ++ l2)
+    | _      , _       => None
+    end
+  | _           => None
+  end
+end.
+
+Fixpoint pat_vars (p : Pat) : nat :=
+match p with
+ | PLit _ => 0
+ | PPid _ => 0
+ | PVar => 1
+ | PNil => 0
+ | PCons p1 p2 => pat_vars p1 + pat_vars p2
+end.
+
+Lemma match_pattern_length : forall p v l,
+  match_pattern p v = Some l -> pat_vars p = length l.
+Proof.
+  induction p; intros.
+  * simpl in *. destruct v; inversion H. break_match_hyp; now inversion H.
+  * simpl in *. destruct v; inversion H. break_match_hyp; now inversion H.
+  * simpl in *. destruct v; inversion H; subst; auto.
+  * simpl in *. destruct v; inversion H. subst. auto.
+  * simpl. simpl in H. destruct v; try congruence.
+    break_match_hyp; try congruence. break_match_hyp; try congruence. inversion H.
+    subst. erewrite length_app, IHp1, IHp2. reflexivity. all: eauto.
+Qed.
+
