src/SyntaxBasics.v
@@ -1,0 +1,55 @@
+From CoreErlang Require Export Basics.
+
+(** Process identifiers are regarded as nats *)
+Definition PID : Set := nat.
+
+(** Currently, we include atoms and integers as literals. We note that 
+    atoms are also used for built-in function names.
+*)
+Inductive Lit : Set :=
+| Atom (s : string)
+| Int (z : Z).
+
+(** Coercions to be able to write down literals in a simpler way. *)
+Coercion Atom : string >-> Lit.
+Coercion Int  : Z >-> Lit.
+
+(** Patterns are the following contructs. Patterns variables in Core
+    Erlang are unique, they can appear at most once in any Pattern.
+    Because of this, in the nameless representation, no indices
+    are needed for pattern variables.
+
+    For technical reasons, PIDs are included as patterns, but they could
+    be omitted by implementing the function erlang:is_pid/1.
+
+    We note, that this resriction is not applicable for Erlang, though.
+*)
+Inductive Pat : Set :=
+| PLit (l : Lit)
+| PPid (p : PID)
+| PVar (** will be assigned in increasing order *)
+| PNil
+| PCons (p1 p2 : Pat).
+
+
+
+Definition lit_eqb (l1 l2 : Lit) : bool :=
+match l1, l2 with
+ | Atom s, Atom s2 => String.eqb s s2
+ | Int z , Int z2  => Z.eqb z z2
+ | _     , _       => false
+end.
+
+Lemma lit_eqb_eq : forall l1 l2, lit_eqb l1 l2 = true <-> l1 = l2.
+Proof.
+  destruct l1, l2; split; intros; subst; auto; simpl in H; try congruence.
+  * apply eqb_eq in H. now inversion H.
+  * inversion H. subst. simpl. now rewrite eqb_refl.
+  * apply Z.eqb_eq in H. now inversion H.
+  * inversion H. subst. simpl. now rewrite Z.eqb_refl.
+Qed.
+
+Lemma lit_eqb_refl : forall l, lit_eqb l l = true.
+Proof.
+  intro. rewrite lit_eqb_eq. reflexivity.
+Qed.
